LeanYjs/Network/CausalNetwork.lean
@@ -1,0 +1,191 @@
+import Init.Data
+
+import LeanYjs.ClientId
+import LeanYjs.Network.CausalOrder
+
+namespace Network
+
+class Message (A : Type) where
+  messageId : A → String
+
+inductive Event (A : Type) : Type where
+  | Broadcast : A → Event A
+  | Deliver : A → Event A
+  deriving Inhabited, Repr, BEq, DecidableEq, Hashable
+
+def Event.id {A} [Message A] : Event A → String
+  | Event.Broadcast a => Message.messageId a
+  | Event.Deliver a => Message.messageId a
+
+structure NodeHistories (E : Type) where
+  histories : ClientId → List E
+  event_distinct : forall i, (histories i).Nodup
+
+def locallyOrdered {E} [DecidableEq E] (histories : NodeHistories E) (i : ClientId) (e1 e2 : E) : Prop :=
+  ∃ l1 l2 l3, histories.histories i = l1 ++ [e1] ++ l2 ++ [e2] ++ l3
+
+structure NetworkBase A [DecidableEq A] [Message A] extends NodeHistories (Event A) where
+  deliver_has_a_cause : forall {i e}, Event.Deliver e ∈ histories i → ∃ j, Event.Broadcast e ∈ histories j
+  deliver_locally : forall {i e}, Event.Deliver e ∈ histories i →
+    locallyOrdered toNodeHistories i (Event.Broadcast e) (Event.Deliver e)
+  msg_id_unique : forall {mi mj i j}, Event.Broadcast mi ∈ histories i → Event.Broadcast mj ∈ histories j → Message.messageId mi = Message.messageId mj → i = j ∧ mi = mj
+
+inductive HappensBefore {A} [DecidableEq A] [Message A] (network : NetworkBase A) : A → A → Prop
+  | broadcast_broadcast_local : locallyOrdered network.toNodeHistories i (Event.Broadcast e1) (Event.Broadcast e2) → HappensBefore network e1 e2
+  | broadcast_deliver_local : locallyOrdered network.toNodeHistories i (Event.Broadcast e1) (Event.Deliver e2) → HappensBefore network e1 e2
+  | trans : HappensBefore network e1 e2 → HappensBefore network e2 e3 → HappensBefore network e1 e3
+
+structure CausalNetwork A [DecidableEq A] [Message A] extends NetworkBase A where
+  causal_delivery : forall {i e1 e2}, Event.Deliver e2 ∈ histories i → HappensBefore toNetworkBase e1 e2 → locallyOrdered toNodeHistories i (Event.Deliver e1) (Event.Deliver e2)
+  -- This assumption is not assumed in the paper, but it is necessary for the ensuring total order of Yjs items and for my proof.
+  -- It is also a reasonable assumption because in a real Yjs implementation, a client would apply item same time at the time of creation of the item by library API (e.g., insert).
+  histories_deliver_broadcast_ordered : forall (e1 e2 : A) i,
+    locallyOrdered toNodeHistories i (Event.Broadcast e1) (Event.Broadcast e2) →
+    locallyOrdered toNodeHistories i (Event.Deliver e1) (Event.Broadcast e2)
+
+structure CausalNetworkElem A [DecidableEq A] [Message A] (network : CausalNetwork A) where
+  elem : A
+
+instance instCausalNetworkElemCausalOrder [DecidableEq A] [Message A] (network : CausalNetwork A) : CausalOrder (CausalNetworkElem A network) where
+  lt a b := HappensBefore network.toNetworkBase a.elem b.elem
+  le a b := a = b ∨ HappensBefore network.toNetworkBase a.elem b.elem
+  le_refl := fun a => Or.inl rfl
+  le_trans := fun a b c h_ab h_bc => by
+    cases h_ab with
+    | inl h_eq =>
+      subst h_eq
+      assumption
+    | inr h_hb_ab =>
+      cases h_bc with
+      | inl h_eq =>
+        subst h_eq
+        right; assumption
+      | inr h_hb_bc =>
+        right
+        apply HappensBefore.trans h_hb_ab h_hb_bc
+  le_antisymm := fun a b h_ab h_ba => by
+    suffices HappensBefore network.toNetworkBase a.elem b.elem → HappensBefore network.toNetworkBase b.elem a.elem → False by
+      cases h_ab with
+      | inl h_eq => assumption
+      | inr h_hb_ab =>
+        cases h_ba with
+        | inl h_eq =>
+          subst h_eq
+          simp
+        | inr h_hb_ba =>
+          exfalso
+          apply this h_hb_ab h_hb_ba
+    intros h_ab h_ba
+    -- suppose a < a
+    -- if a < a only consists of broadcast_deliver_local, then we can conclude a.idx < a.idx, which is a contradiction
+    -- otherwise, if a < a is break down into a < b and b < a and a < b is broadcast_deliver_local, we now have
+    -- D(a) <_i B(b) and b < a.
+    -- so by causal_delivery, we have D(b) <_i D(a), but it followed by D(b) <_i B(b), it contradicts with deliver_locally.
+    sorry
+  lt_iff_le_not_ge := by sorry
+
+section OperationNetwork
+
+variable [Operation A] [Message A] [DecidableEq A]
+variable (network : CausalNetwork A)
+
+def CausalNetwork.toDeliverMessages (network : CausalNetwork A) (i : ClientId) : List (CausalNetworkElem A network) :=
+  network.toNodeHistories.histories i |>.filterMap (fun ev => match ev with
+    | Event.Deliver a => some (CausalNetworkElem.mk a)
+    | _ => none)
+
+-- don't need induction because it is sufficient to use filterMap_eq_..._iff lemma
+omit [Operation A] in theorem toDeliverMessages_histories (i : ClientId) :
+  network.toDeliverMessages i = l1 ++ [m] ++ l2 ++ [m'] ++ l3 →
+  ∃ l1 l2 l3,
+    network.toNodeHistories.histories i = l1 ++ [Event.Deliver m.elem] ++ l2 ++ [Event.Deliver m'.elem] ++ l3 := by
+  intro h_deliver_msgs
+  simp [CausalNetwork.toDeliverMessages] at h_deliver_msgs
+  generalize network.toNodeHistories.histories i = history at *
+  induction history generalizing l1 m l2 m' l3 with
+  | nil =>
+    simp at h_deliver_msgs
+  | cons ev history ih =>
+    cases ev with
+    | Broadcast a =>
+      simp [List.filterMap_cons_none] at h_deliver_msgs
+      obtain ⟨ l1', m'', l2', m''', l3', h_eq ⟩ := ih h_deliver_msgs
+      use (Event.Broadcast a :: l1'), m'', l2'
+      simp
+    | Deliver a =>
+      simp at h_deliver_msgs
+      cases l1 with
+      | cons x l1 =>
+        simp at h_deliver_msgs
+        replace ⟨ _, h_deliver_msgs ⟩ := h_deliver_msgs
+        obtain ⟨ l1', m'', l2', m''', l3', h_eq ⟩ := ih h_deliver_msgs
+        use (Event.Deliver a :: l1'), m'', l2'
+        simp
+      | nil =>
+        simp at h_deliver_msgs
+        obtain ⟨ h_m_eq, h_deliver_msgs ⟩ := h_deliver_msgs
+        use []
+        simp
+        rw [List.filterMap_eq_append_iff] at h_deliver_msgs
+        obtain ⟨ l2', l3', h_eq', h_eq2', h_eq3' ⟩ := h_deliver_msgs
+        rw [List.filterMap_eq_cons_iff] at h_eq3'
+        obtain ⟨ l3', y, h_eq3', l3'', h_none, h_some, h_filterMap ⟩ := h_eq3'
+        subst history l3''
+        constructor
+        . subst m; simp
+        . use (l2' ++ l3'), h_eq3'
+          simp
+          cases y with
+          | Broadcast a' =>
+            simp at h_some
+          | Deliver a' =>
+            simp at h_some
+            subst m'
+            simp
+
+theorem hb_consistent_local_history_aux i ms ms' :
+  ms ++ ms' = network.toDeliverMessages i →
+  hb_consistent (hb := instCausalNetworkElemCausalOrder network) ms' := by
+  intros h_ms
+  -- simp [CausalNetwork.toDeliverMessages] at h_ms
+  induction ms' generalizing ms with
+  | nil =>
+    simp [hb_consistent.nil]
+  | cons h t ih =>
+    conv at h_ms =>
+      lhs
+      rw [List.append_cons]
+      rfl
+    apply hb_consistent.cons
+    . apply ih (ms ++ [h]) h_ms
+    . intros m h_mem h_le
+      cases h_le with
+      | inr h_lt =>
+        have ⟨ t1, t2, h_t_eq ⟩ : ∃ t1 t2, t = t1 ++ [m] ++ t2 := by
+          rw [List.mem_iff_append] at h_mem
+          simp
+          assumption
+        subst h_t_eq
+        replace h_ms : network.toDeliverMessages i =  ms ++ [h] ++ t1 ++ [m] ++ t2 := by
+          rw [←h_ms]
+          simp
+        obtain ⟨ l1, l2, l3, h_history_eq ⟩ := toDeliverMessages_histories network i h_ms
+        have h_locally_ordered : locallyOrdered network.toNodeHistories i (Event.Deliver h.elem) (Event.Deliver m.elem) := by
+          simp [locallyOrdered]
+          use l1, l2, l3
+          rw [h_history_eq]
+          simp
+        apply network.causal_delivery (i := i) at h_lt
+        . -- need locallyOrdered asym
+          sorry
+        . sorry
+      | inl h_eq =>
+        sorry
+
+theorem hb_consistent_local_history i :
+  hb_consistent (hb := instCausalNetworkElemCausalOrder network) (network.toDeliverMessages i) := by
+  apply hb_consistent_local_history_aux network i []
+  simp
+end OperationNetwork
+
+end Network
